common/Globalenvs.v
@@ -82,6 +82,7 @@ Module Genv (P:Policy) (A:Allocator P).
                                                                   block (functions) or
                                                                   base, bound, tag *)
       genv_fun_defs: PTree.t (globdef F V);                    (**r mapping block -> definition *)
+      genv_ef_defs: PTree.t (external_function * typelist * type * calling_convention);
       genv_next_block: block;                                  (**r next block for functions *)
     }.
 
@@ -133,29 +134,34 @@ Module Genv (P:Policy) (A:Allocator P).
     Definition find_funct_ptr (ge: t) (b: block) : option F :=
       match PTree.get b ge.(genv_fun_defs) with Some (Gfun f) => Some f | _ => None end.
 
+    Definition find_ef_ptr (ge: t) (b: block) :
+      option (external_function * typelist * type * calling_convention) :=
+      PTree.get b ge.(genv_ef_defs).
+    
     (** [find_funct] is similar to [find_funct_ptr], but the function address
         is given as a value. *)
-    Definition find_funct (ge: t) (v: val) : option F :=
+    Definition find_funct (ge: t) (v: val) : option (fundef F) :=
       match v with
       | Vfptr b =>
-          find_funct_ptr ge b
+          match find_funct_ptr ge b with
+          | Some fd => Some (Internal fd)
+          | None => match find_ef_ptr ge b with
+                    | Some (ef,tyargs,tyres,cc) => Some (External ef tyargs tyres cc)
+                    | None => None
+                    end
+          end
       | _ => None
       end.
+
+    Definition invert_ef (ge: t) (ef: external_function) : option ident :=
+      PTree.fold
+        (fun res id '(ef',tyargs,tyres,cc) =>
+           if external_function_eq ef ef' then Some id else res)
+        ge.(genv_ef_defs) None.      
     
     (** ** Constructing the global environment *)
 
     Section CONSTRUCTION.
-
-  (*Function store_zeros (m: mem) (p: Z) (n: Z) {wf (Zwf 0) n}: MemoryResult mem :=
-    if zle n 0 then MemorySuccess m else
-      match Mem.store Mint8unsigned m p (Vzero, def_tag) [def_tag] with
-      | MemorySuccess m' => store_zeros m' (p + 1) (n - 1)
-      | res => res
-      end.
-  Proof.
-    intros. red. lia.
-    apply Zwf_well_founded.
-  Qed.*)
 
       Definition store_init_data (ge: t) (m: mem) (p: Z) (id: init_data) (vt: tag) (lt: tag) :
         MemoryResult mem :=
@@ -222,7 +228,8 @@ Module Genv (P:Policy) (A:Allocator P).
                              ge.(genv_public)
                                   genv_symb'
                                   ge.(genv_fun_defs)
-                                       ge.(genv_next_block)
+                                  ge.(genv_ef_defs)
+                                  ge.(genv_next_block)
                 in
                 (ge', m')
             | MemoryFail msg failure => (ge, m)
@@ -232,6 +239,7 @@ Module Genv (P:Policy) (A:Allocator P).
                          ge.(genv_public)
                               (PTree.set idg#1 (inl (ge.(genv_next_block), def_tag)) ge.(genv_symb))
                                    (PTree.set ge.(genv_next_block) idg#2 ge.(genv_fun_defs))
+                                   ge.(genv_ef_defs)
                                    (Pos.succ ge.(genv_next_block))
             in
             (ge', m)
@@ -242,12 +250,23 @@ Module Genv (P:Policy) (A:Allocator P).
         match gl with
         | [] => (ge,m)
         | g::gl' =>
-            let '(ge', m') := add_global ge m tree g in
-            add_globals ge' m' tree gl'
+            let '(ge', m') := add_globals ge m tree gl' in
+            add_global ge' m' tree g
+        end.
+
+      Fixpoint add_builtins (ge: t)
+               (el: list (ident*external_function*typelist*type*calling_convention)) : t :=
+        match el with
+        | [] => ge
+        | (id, ef, tyargs, tyres, cc) :: el' =>
+            let ge' := @mkgenv ge.(genv_public) ge.(genv_symb) ge.(genv_fun_defs)
+                               (PTree.set id (ef,tyargs,tyres,cc) ge.(genv_ef_defs))
+                               ge.(genv_next_block) in
+            add_builtins ge el'
         end.
       
       Program Definition empty_genv (pub: list ident): t :=
-        @mkgenv pub (PTree.empty _) (PTree.empty _) 2%positive.
+        @mkgenv pub (PTree.empty _) (PTree.empty _) (PTree.empty _) 2%positive.
 
       Definition init_record (m: A.mem) (base: Z) (sz: Z) : MemoryResult A.mem :=
         let szv := Vlong (Int64.neg (Int64.repr sz)) in
@@ -260,7 +279,7 @@ Module Genv (P:Policy) (A:Allocator P).
         | _::idgs' => filter_var_sizes idgs'
         end.
       
-      Definition globalenv (p: AST.program F V) :=
+      Definition globalenv (p: AST.program F V) : MemoryResult (t * mem) :=
         match init_record A.empty 1000 1000 with
         | MemorySuccess m =>
             let (m',tree) := A.globalalloc m (filter_var_sizes p.(AST.prog_defs)) in
@@ -301,32 +320,6 @@ Module Genv (P:Policy) (A:Allocator P).
           | i :: il => bytes_of_init_data ge i t ++ bytes_of_init_data_list il t
           end.
 
-(*Lemma store_init_data_list_loadbytes:
-  forall b il m p m',
-  store_init_data_list m b p il = Some m' ->
-  readbytes_as_zero m b p (init_data_list_size il) ->
-  Mem.loadbytes m' b p (init_data_list_size il) = Some (bytes_of_init_data_list il).
-Proof.
-  induction il as [ | i1 il]; simpl; intros.
-- apply Mem.loadbytes_empty. lia.
-- generalize (init_data_size_pos i1) (init_data_list_size_pos il); intros P1 PL.
-  destruct (store_init_data m b p i1) as [m1|] eqn:S; try discriminate.
-  apply Mem.loadbytes_concat.
-  eapply Mem.loadbytes_unchanged_on with (P := fun b1 ofs1 => ofs1 < p + init_data_size i1).
-  eapply store_init_data_list_unchanged; eauto.
-  intros; lia.
-  intros; lia.
-  eapply store_init_data_loadbytes; eauto.
-  red; intros; apply H0. lia. lia.
-  apply IHil with m1; auto.
-  red; intros.
-  eapply Mem.loadbytes_unchanged_on with (P := fun b1 ofs1 => p + init_data_size i1 <= ofs1).
-  eapply store_init_data_unchanged; eauto.
-  intros; lia.
-  intros; lia.
-  apply H0. lia. lia.
-  auto. auto.
-Qed.*)
         End WITH_GE.
     End CONSTRUCTION.
       
@@ -349,119 +342,50 @@ Qed.*)
       intros. exists b; congruence.
     Qed.
 
-    Theorem find_funct_find_funct_ptr:
-      forall ge b,
-        find_funct ge (Vfptr b) = find_funct_ptr ge b.
-    Proof.
-      intros; auto.
-    Qed.
-
-(*    Theorem find_var_info_iff:
-      forall ge ofs v, find_var_info ge ofs = Some v <-> find_def ge ofs = Some (Gvar v).
-    Proof.
-      intros. unfold find_var_info. destruct (find_def ge) as [[f1|v1]|]; intuition congruence.
-    Qed. *)
-
-    Theorem find_symbol_exists:
-      forall p id g ge m,
-        In (id, g) (AST.prog_defs p) ->
+    Corollary find_funct_ptr_inversion:
+      forall p b f ge m,
         globalenv p = MemorySuccess (ge,m) ->
-        exists b, find_symbol ge id = Some b.
+        find_funct_ptr ge b = Some f ->
+        In (b, Gfun f) (AST.prog_defs p).
+(*    Proof.
+      destruct p. induction prog_defs; intros.
+      - unfold globalenv in *. destruct (init_record Genv.empty 1000 1000); inv H.
+        destruct (globalalloc a []); inv H2.
+        inv H0.
+      - destruct a. destruct g.
+        + destruct (Pos.eq_dec b i); destruct (F_eq_dec f f0).
+          * left. subst. auto.
+          * simpl in *. right. unfold find_funct_ptr in H0.
+            unfold genv_fun_defs in H0. destruct ge.
+            
+            unfold globalenv in *. unfold filter_var_sizes in *.
+            simpl in *.
+            destruct (init_record Genv.empty 1000 1000); inv H.
+            unfold empty_genv in *. 
+            destruct (globalalloc a (filter_var_sizes prog_defs)); inv H2.
+            destruct (add_globals (empty_genv prog_public) a t0 prog_defs).
+            destruct (add_global t1 m1 t0 (i, Gfun f0)).
+            eapply IHprog_defs. reflexivity.
+        destruct (Pos.eq_dec b i).
+        + destruct (globdef_eq_dec (Gfun f) g).
+          * subst. left. auto.
+          * right. apply IHprog_defs. rewrite <- H1.
+            simpl. unfold add_global.
+        + right.
+    Qed.*)
     Admitted.
-(*Proof.
-  intros. unfold globalenv. eapply add_globals_ensures; eauto.
-(* preserves *)
-  intros. unfold find_symbol; simpl. rewrite PTree.gsspec. destruct (peq id id0).
-  econstructor; eauto.
-  auto.
-(* ensures *)
-  intros. unfold find_symbol; simpl. rewrite PTree.gss. econstructor; eauto.
-Qed.*)
-
-      Theorem find_symbol_inversion : forall p x b,
-        forall ge m,
-          globalenv p = MemorySuccess (ge,m) ->
-          find_symbol ge x = Some b ->
-          In x (prog_defs_names p).
-      Admitted.
-(*Proof.
-  intros until b; unfold globalenv. eapply add_globals_preserves.
-(* preserves *)
-  unfold find_symbol; simpl; intros. rewrite PTree.gsspec in H1.
-  destruct (peq x id). subst x. change id with (fst (id, g)). apply List.in_map; auto.
-  auto.
-(* base *)
-  unfold find_symbol; simpl; intros. rewrite PTree.gempty in H. discriminate.
-Qed.*)
-
-(*      Theorem find_def_inversion:
-        forall p ofs g ge m,
-          globalenv p = (ge,m) ->
-          find_def ge ofs = Some g ->
-          exists id, In (id, g) (AST.prog_defs p).
-      Admitted. *)
-(*Proof.
-  intros until g. unfold globalenv. apply add_globals_preserves.
-(* preserves *)
-  unfold find_def; simpl; intros.
-  rewrite PTree.gsspec in H1. destruct (peq b (genv_next ge)).
-  inv H1. exists id; auto.
-  auto.
-(* base *)
-  unfold find_def; simpl; intros. rewrite PTree.gempty in H. discriminate.
-Qed.*)
-
-      Corollary find_funct_ptr_inversion:
-        forall p b f ge m,
-          globalenv p = MemorySuccess (ge,m) ->
-          find_funct_ptr ge b = Some f ->
-          exists id, In (id, Gfun f) (AST.prog_defs p).
-      Admitted.
-      (*Proof.
-        intros. apply find_def_inversion with b. apply find_funct_ptr_iff; auto.
-        Qed.*)  
-
-      Corollary find_funct_inversion:
-        forall p v f ge m,
-          globalenv p = MemorySuccess (ge,m) ->
-          find_funct ge v = Some f ->
-          exists id, In (id, Gfun f) (AST.prog_defs p).
-      Proof.
-        intros. exploit find_funct_inv; eauto. intros [b EQ]. subst v.
-        rewrite find_funct_find_funct_ptr in H0.
-        eapply find_funct_ptr_inversion; eauto.
-      Qed.
-
-      Theorem find_funct_ptr_prop:
-        forall (P: F -> Prop) p b f ge m,
-          globalenv p = MemorySuccess (ge,m) ->
-          (forall id f, In (id, Gfun f) (AST.prog_defs p) -> P f) ->
-          find_funct_ptr ge b = Some f ->
-          P f.
-      Proof.
-        intros. exploit find_funct_ptr_inversion; eauto. intros [id IN]. eauto.
-      Qed.
-
-      Theorem find_funct_prop:
-        forall (P: F -> Prop) p v f ge m,
-          globalenv p = MemorySuccess (ge,m) ->
-          (forall id f, In (id, Gfun f) (AST.prog_defs p) -> P f) ->
-          find_funct ge v = Some f ->
-          P f.
-      Proof.
-        intros. exploit find_funct_inversion; eauto. intros [id IN]. eauto.
-      Qed.
-
-(*Theorem global_addresses_distinct:
-  forall ge id1 id2 b1 b2,
-  id1 <> id2 ->
-  find_symbol ge id1 = Some b1 ->
-  find_symbol ge id2 = Some b2 ->
-  b1 <> b2.
-Proof.
-  intros. red; intros; subst. elim H. destruct ge. eauto.
-Qed.*)
-
+    
+(*    Corollary find_funct_inversion:
+      forall p v f ge m,
+        globalenv p = MemorySuccess (ge,m) ->
+        find_funct ge v = Some f ->
+        exists id, In (id, Gfun f) (AST.prog_defs p).
+    Proof.
+      intros. exploit find_funct_inv; eauto. intros [b EQ]. subst v.
+      exists b. rewrite find_funct_find_funct_ptr in H0.
+      eapply find_funct_ptr_inversion; eauto.
+    Qed. *)
+        
       Theorem invert_find_symbol_block:
         forall ge id b,
           invert_symbol_block ge b = Some id ->
@@ -514,403 +438,7 @@ Qed.*)
           find_symbol ge id = Some (inl (b,t)) ->
           invert_symbol_block ge b = Some id.
       Admitted.
-
-(*Remark store_init_data_perm:
-  forall prm b' q i vt lts b m p m',
-  store_init_data m b p i vt lts = Some m' ->
-  (Mem.perm m b' q prm <-> Mem.perm m' b' q prm).
-Proof.
-  intros.
-  assert (forall chunk v vt lts,
-          Mem.store chunk m b p (v, vt) lts = Some m' ->
-          (Mem.perm m b' q prm <-> Mem.perm m' b' q prm)).
-    intros; split; eauto with mem.
-  destruct i; simpl in H; eauto.
-  inv H; tauto.
-  destruct (find_symbol ge i); try discriminate. destruct p0. eauto.
-Qed.*)
-
-(*Remark store_init_data_list_perm:
-  forall prm q idl m p m',
-  store_init_data_list m p idl = MemorySuccess m' ->
-  (Mem.perm m q prm <-> Mem.perm m' q prm).
-Admitted.*)
-(*Proof.
-  induction idl as [ | i1 idl]; simpl; intros.
-- inv H; tauto.
-- destruct (store_init_data m b p i1) as [m1|] eqn:S1; try discriminate.
-  transitivity (Mem.perm m1 b' q prm).
-  eapply store_init_data_perm; eauto.
-  eapply IHidl; eauto.
-Qed.*)
-
-(*Remark alloc_global_perm:
-  forall prm b' q idg m m',
-  alloc_global m idg = Some m' ->
-  Mem.valid_block m b' ->
-  (Mem.perm m b' q prm <-> Mem.perm m' b' q prm).
-Proof.
-  intros. destruct idg as [id [f|v]]; simpl in H.
-  (* function *)
-  destruct (Mem.alloc m 0 1) as [m1 b] eqn:?.
-  assert (b' <> b). apply Mem.valid_not_valid_diff with m; eauto with mem.
-  split; intros.
-  eapply Mem.perm_drop_3; eauto. eapply Mem.perm_alloc_1; eauto.
-  eapply Mem.perm_alloc_4; eauto. eapply Mem.perm_drop_4; eauto.
-  (* variable *)
-  set (init := gvar_init v) in *.
-  set (sz := init_data_list_size init) in *.
-  destruct (Mem.alloc m 0 sz) as [m1 b] eqn:?.
-  destruct (store_zeros m1 b 0 sz) as [m2|] eqn:?; try discriminate.
-  destruct (store_init_data_list m2 b 0 init) as [m3|] eqn:?; try discriminate.
-  assert (b' <> b). apply Mem.valid_not_valid_diff with m; eauto with mem.
-  split; intros.
-  eapply Mem.perm_drop_3; eauto.
-  erewrite <- store_init_data_list_perm; [idtac|eauto].
-  erewrite <- store_zeros_perm; [idtac|eauto].
-  eapply Mem.perm_alloc_1; eauto.
-  eapply Mem.perm_alloc_4; eauto.
-  erewrite store_zeros_perm; [idtac|eauto].
-  erewrite store_init_data_list_perm; [idtac|eauto].
-  eapply Mem.perm_drop_4; eauto.
-Qed.*)
-
-(*Remark alloc_globals_perm:
-  forall prm b' q gl m m',
-  alloc_globals m gl = Some m' ->
-  Mem.valid_block m b' ->
-  (Mem.perm m b' q prm <-> Mem.perm m' b' q prm).
-Proof.
-  induction gl.
-  simpl; intros. inv H. tauto.
-  simpl; intros. destruct (alloc_global m a) as [m1|] eqn:?; try discriminate.
-  erewrite alloc_global_perm; eauto. eapply IHgl; eauto.
-  unfold Mem.valid_block in *. erewrite alloc_global_nextblock; eauto.
-  apply Plt_trans_succ; auto.
-Qed.*)
-
-
-(** Properties related to [load] *)
-
-      Definition read_as_zero (m: mem) (ofs len: Z) : Prop :=
-        forall chunk p,
-          ofs <= p -> p + size_chunk chunk <= ofs + len ->
-          (align_chunk chunk | p) ->
-          exists t,
-            load chunk m p =
-              MemorySuccess (match chunk with
-                             | Mint8unsigned | Mint8signed | Mint16unsigned | Mint16signed | Mint32 => Vint Int.zero
-                             | Mint64 => Vlong Int64.zero
-                             | Mfloat32 => Vsingle Float32.zero
-                             | Mfloat64 => Vfloat Float.zero
-                             | Many32 | Many64 => Vundef
-                             end,t).
-
-(*Fixpoint load_store_init_data (m: mem) (p: Z) (il: list init_data) (t:tag) {struct il} : Prop :=
-  match il with
-  | nil => True
-  | Init_int8 n :: il' =>
-      Mem.load Mint8unsigned m p = Some(Vint(Int.zero_ext 8 n),t)
-      /\ load_store_init_data m (p + 1) il' t
-  | Init_int16 n :: il' =>
-      Mem.load Mint16unsigned m p = Some(Vint(Int.zero_ext 16 n),t)
-      /\ load_store_init_data m (p + 2) il' t
-  | Init_int32 n :: il' =>
-      Mem.load Mint32 m p = Some(Vint n,t)
-      /\ load_store_init_data m (p + 4) il' t
-  | Init_int64 n :: il' =>
-      Mem.load Mint64 m p = Some(Vlong n,t)
-      /\ load_store_init_data m (p + 8) il' t
-  | Init_float32 n :: il' =>
-      Mem.load Mfloat32 m p = Some(Vsingle n,t)
-      /\ load_store_init_data m (p + 4) il' t
-  | Init_float64 n :: il' =>
-      Mem.load Mfloat64 m p = Some(Vfloat n,t)
-      /\ load_store_init_data m (p + 8) il' t
-  | Init_addrof symb ofs :: il' =>
-      (exists b' base bound pt, find_symbol ge symb = Some (b',base,bound,pt) /\ Mem.load Mptr m p = Some (Vptr b' ofs,t))
-      /\ load_store_init_data m b (p + size_chunk Mptr) il' t
-  | Init_space n :: il' =>
-      read_as_zero m b p n
-      /\ load_store_init_data m b (p + Z.max n 0) il' t
-  end.*)
-
-(*Lemma store_init_data_list_charact:
-  forall b il m p m',
-  store_init_data_list m b p il = Some m' ->
-  read_as_zero m b p (init_data_list_size il) ->
-  load_store_init_data m' b p il.
-Proof.
-  assert (A: forall chunk v m b p m1 il m',
-    Mem.store chunk m b p v = Some m1 ->
-    store_init_data_list m1 b (p + size_chunk chunk) il = Some m' ->
-    Mem.load chunk m' b p = Some(Val.load_result chunk v)).
-  {
-    intros.
-    eapply Mem.load_unchanged_on with (P := fun b' ofs' => ofs' < p + size_chunk chunk).
-    eapply store_init_data_list_unchanged; eauto. intros; lia.
-    intros; tauto.
-    eapply Mem.load_store_same; eauto.
-  }
-  induction il; simpl.
-- auto.
-- intros. destruct (store_init_data m b p a) as [m1|] eqn:?; try congruence.
-  exploit IHil; eauto.
-  set (P := fun (b': block) ofs' => p + init_data_size a <= ofs').
-  apply read_as_zero_unchanged with (m := m) (P := P).
-  red; intros; apply H0; auto. generalize (init_data_size_pos a); lia. lia.
-  eapply store_init_data_unchanged with (P := P); eauto.
-  intros; unfold P. lia.
-  intros; unfold P. lia.
-  intro D.
-  destruct a; simpl in Heqo.
-+ split; auto. eapply (A Mint8unsigned (Vint i)); eauto.
-+ split; auto. eapply (A Mint16unsigned (Vint i)); eauto.
-+ split; auto. eapply (A Mint32 (Vint i)); eauto.
-+ split; auto. eapply (A Mint64 (Vlong i)); eauto.
-+ split; auto. eapply (A Mfloat32 (Vsingle f)); eauto.
-+ split; auto. eapply (A Mfloat64 (Vfloat f)); eauto.
-+ split; auto.
-  set (P := fun (b': block) ofs' => ofs' < p + init_data_size (Init_space z)).
-  inv Heqo. apply read_as_zero_unchanged with (m := m1) (P := P).
-  red; intros. apply H0; auto. simpl. generalize (init_data_list_size_pos il); extlia.
-  eapply store_init_data_list_unchanged; eauto.
-  intros; unfold P. lia.
-  intros; unfold P. simpl; extlia.
-+ rewrite init_data_size_addrof in *.
-  split; auto.
-  destruct (find_symbol ge i); try congruence.
-  exists b0; split; auto.
-  transitivity (Some (Val.load_result Mptr (Vptr b0 i0))).
-  eapply (A Mptr (Vptr b0 i0)); eauto.
-  unfold Val.load_result, Mptr; destruct Archi.ptr64; auto.
-Qed.*)
-
-(*Remark alloc_global_unchanged:
-  forall (P: block -> Z -> Prop) m id g m',
-  alloc_global m (id, g) = Some m' ->
-  Mem.unchanged_on P m m'.
-Proof.
-  intros. destruct g as [f|v]; simpl in H.
-- (* function *)
-  destruct (Mem.alloc m 0 1) as [m1 b] eqn:?.
-  set (Q := fun b' (ofs: Z) => b' <> b).
-  apply Mem.unchanged_on_implies with Q.
-  apply Mem.unchanged_on_trans with m1.
-  eapply Mem.alloc_unchanged_on; eauto.
-  eapply Mem.drop_perm_unchanged_on; eauto.
-  intros; red. apply Mem.valid_not_valid_diff with m; eauto with mem.
-- (* variable *)
-  set (init := gvar_init v) in *.
-  set (sz := init_data_list_size init) in *.
-  destruct (Mem.alloc m 0 sz) as [m1 b] eqn:?.
-  destruct (store_zeros m1 b 0 sz) as [m2|] eqn:?; try discriminate.
-  destruct (store_init_data_list m2 b 0 init) as [m3|] eqn:?; try discriminate.
-  set (Q := fun b' (ofs: Z) => b' <> b).
-  apply Mem.unchanged_on_implies with Q.
-  apply Mem.unchanged_on_trans with m1.
-  eapply Mem.alloc_unchanged_on; eauto.
-  apply Mem.unchanged_on_trans with m2.
-  eapply store_zeros_unchanged; eauto.
-  apply Mem.unchanged_on_trans with m3.
-  eapply store_init_data_list_unchanged; eauto.
-  eapply Mem.drop_perm_unchanged_on; eauto.
-  intros; red. apply Mem.valid_not_valid_diff with m; eauto with mem.
-Qed.*)
-
-(*Remark alloc_globals_unchanged:
-  forall (P: block -> Z -> Prop) gl m m',
-  alloc_globals m gl = Some m' ->
-  Mem.unchanged_on P m m'.
-Proof.
-  induction gl; simpl; intros.
-- inv H. apply Mem.unchanged_on_refl.
-- destruct (alloc_global m a) as [m''|] eqn:?; try discriminate.
-  destruct a as [id g].
-  apply Mem.unchanged_on_trans with m''.
-  eapply alloc_global_unchanged; eauto.
-  apply IHgl; auto.
-Qed.*)
-
-(*Remark load_store_init_data_invariant:
-  forall m m' b t,
-    (forall chunk ofs, Mem.load chunk m' b ofs = Mem.load chunk m b ofs) ->
-    forall il p,
-      load_store_init_data m b p il t -> load_store_init_data m' b p il t.
-Proof.
-  induction il; intro p; simpl.
-  auto.
-  rewrite ! H. destruct a; intuition. red; intros; rewrite H; auto.
-Qed.*)
-
-(*Definition globals_initialized (g: t) (m: mem) :=
-  forall b gd,
-  find_def g b = Some gd ->
-  match gd with
-  | Gfun f =>
-         Mem.perm m b 0 Live
-      /\ (forall ofs p, Mem.perm m b ofs p -> ofs = 0 /\ p = Nonempty)
-  | Gvar v =>
-         Mem.range_perm m b 0 (init_data_list_size v.(gvar_init)) Cur (perm_globvar v)
-      /\ (forall ofs p, Mem.perm m b ofs p ->
-            0 <= ofs < init_data_list_size v.(gvar_init) /\ perm_order (perm_globvar v) p)
-      /\ (v.(gvar_volatile) = false -> load_store_init_data m b 0 v.(gvar_init))
-      /\ (v.(gvar_volatile) = false -> Mem.loadbytes m b 0 (init_data_list_size v.(gvar_init)) = Some (bytes_of_init_data_list v.(gvar_init)))
-  end.
-
-Lemma alloc_global_initialized:
-  forall g m id gd m',
-  genv_next g = Mem.nextblock m ->
-  alloc_global m (id, gd) = Some m' ->
-  globals_initialized g m ->
-     globals_initialized (add_global g (id, gd)) m'
-  /\ genv_next (add_global g (id, gd)) = Mem.nextblock m'.
-Proof.
-  intros.
-  exploit alloc_global_nextblock; eauto. intros NB. split.
-- (* globals-initialized *)
-  red; intros. unfold find_def in H2; simpl in H2.
-  rewrite PTree.gsspec in H2. destruct (peq b (genv_next g)).
-+ inv H2. destruct gd0 as [f|v]; simpl in H0.
-* destruct (Mem.alloc m 0 1) as [m1 b] eqn:ALLOC.
-  exploit Mem.alloc_result; eauto. intros RES.
-  rewrite H, <- RES. split.
-  eapply Mem.perm_drop_1; eauto. lia.
-  intros.
-  assert (0 <= ofs < 1). { eapply Mem.perm_alloc_3; eauto. eapply Mem.perm_drop_4; eauto. }
-  exploit Mem.perm_drop_2; eauto. intros ORD.
-  split. lia. inv ORD; auto.
-* set (init := gvar_init v) in *.
-  set (sz := init_data_list_size init) in *.
-  destruct (Mem.alloc m 0 sz) as [m1 b] eqn:?.
-  destruct (store_zeros m1 b 0 sz) as [m2|] eqn:?; try discriminate.
-  destruct (store_init_data_list m2 b 0 init) as [m3|] eqn:?; try discriminate.
-  exploit Mem.alloc_result; eauto. intro RES.
-  replace (genv_next g) with b by congruence.
-  split. red; intros. eapply Mem.perm_drop_1; eauto.
-  split. intros.
-  assert (0 <= ofs < sz).
-  { eapply Mem.perm_alloc_3; eauto.
-    erewrite store_zeros_perm by eauto.
-    erewrite store_init_data_list_perm by eauto.
-    eapply Mem.perm_drop_4; eauto. }
-  split; auto.
-  eapply Mem.perm_drop_2; eauto.
-  split. intros NOTVOL. apply load_store_init_data_invariant with m3.
-  intros. eapply Mem.load_drop; eauto. right; right; right.
-  unfold perm_globvar. rewrite NOTVOL. destruct (gvar_readonly v); auto with mem.
-  eapply store_init_data_list_charact; eauto.
-  eapply store_zeros_read_as_zero; eauto.
-  intros NOTVOL.
-  transitivity (Mem.loadbytes m3 b 0 sz).
-  eapply Mem.loadbytes_drop; eauto. right; right; right.
-  unfold perm_globvar. rewrite NOTVOL. destruct (gvar_readonly v); auto with mem.
-  eapply store_init_data_list_loadbytes; eauto.
-  eapply store_zeros_loadbytes; eauto.
-+ assert (U: Mem.unchanged_on (fun _ _ => True) m m') by (eapply alloc_global_unchanged; eauto).
-  assert (VALID: Mem.valid_block m b).
-  { red. rewrite <- H. eapply genv_defs_range; eauto. }
-  exploit H1; eauto.
-  destruct gd0 as [f|v].
-* intros [A B]; split; intros.
-  eapply Mem.perm_unchanged_on; eauto. exact I.
-  eapply B. eapply Mem.perm_unchanged_on_2; eauto. exact I.
-* intros (A & B & C & D). split; [| split; [| split]].
-  red; intros. eapply Mem.perm_unchanged_on; eauto. exact I.
-  intros. eapply B. eapply Mem.perm_unchanged_on_2; eauto. exact I.
-  intros. apply load_store_init_data_invariant with m; auto.
-  intros. eapply Mem.load_unchanged_on_1; eauto. intros; exact I.
-  intros. eapply Mem.loadbytes_unchanged_on; eauto. intros; exact I.
-- simpl. congruence.
-Qed.
-
-Lemma alloc_globals_initialized:
-  forall gl ge m m',
-  alloc_globals m gl = Some m' ->
-  genv_next ge = Mem.nextblock m ->
-  globals_initialized ge m ->
-  globals_initialized (add_globals ge gl) m'.
-Proof.
-  induction gl; simpl; intros.
-- inv H; auto.
-- destruct a as [id g]. destruct (alloc_global m (id, g)) as [m1|] eqn:?; try discriminate.
-  exploit alloc_global_initialized; eauto. intros [P Q].
-  eapply IHgl; eauto.
-Qed.*)
-
-(*Theorem find_symbol_not_fresh:
-  forall p id b m,
-  init_mem p = Some m ->
-  find_symbol (globalenv p) id = Some b -> Mem.valid_block m b.
-Proof.
-  intros. red. erewrite <- init_mem_genv_next; eauto.
-  eapply genv_symb_range; eauto.
-Qed.
-
-Theorem find_def_not_fresh:
-  forall p b g m,
-  init_mem p = Some m ->
-  find_def (globalenv p) b = Some g -> Mem.valid_block m b.
-Proof.
-  intros. red. erewrite <- init_mem_genv_next; eauto.
-  eapply genv_defs_range; eauto.
-Qed.
-
-Theorem find_funct_ptr_not_fresh:
-  forall p b f m,
-  init_mem p = Some m ->
-  find_funct_ptr (globalenv p) b = Some f -> Mem.valid_block m b.
-Proof.
-  intros. rewrite find_funct_ptr_iff in H0. eapply find_def_not_fresh; eauto.
-Qed.
-
-Theorem find_var_info_not_fresh:
-  forall p b gv m,
-  init_mem p = Some m ->
-  find_var_info (globalenv p) b = Some gv -> Mem.valid_block m b.
-Proof.
-  intros. rewrite find_var_info_iff in H0. eapply find_def_not_fresh; eauto.
-Qed.
-
-Lemma init_mem_characterization_gen:
-  forall p m,
-  init_mem p = Some m ->
-  globals_initialized (globalenv p) (globalenv p) m.
-Proof.
-  intros. apply alloc_globals_initialized with Mem.empty.
-  auto.
-  rewrite Mem.nextblock_empty. auto.
-  red; intros. unfold find_def in H0; simpl in H0; rewrite PTree.gempty in H0; discriminate.
-Qed.
-
-Theorem init_mem_characterization:
-  forall p b gv m,
-  find_var_info (globalenv p) b = Some gv ->
-  init_mem p = Some m ->
-  Mem.range_perm m b 0 (init_data_list_size gv.(gvar_init)) Cur (perm_globvar gv)
-  /\ (forall ofs p, Mem.perm m b ofs p ->
-        0 <= ofs < init_data_list_size gv.(gvar_init) /\ perm_order (perm_globvar gv) p)
-  /\ (gv.(gvar_volatile) = false ->
-      load_store_init_data (globalenv p) m b 0 gv.(gvar_init))
-  /\ (gv.(gvar_volatile) = false ->
-      Mem.loadbytes m b 0 (init_data_list_size gv.(gvar_init)) = Some (bytes_of_init_data_list (globalenv p) gv.(gvar_init))).
-Proof.
-  intros. rewrite find_var_info_iff in H.
-  exploit init_mem_characterization_gen; eauto.
-Qed.
-
-Theorem init_mem_characterization_2:
-  forall p b fd m,
-  find_funct_ptr (globalenv p) b = Some fd ->
-  init_mem p = Some m ->
-  Mem.perm m b 0 Cur Nonempty
-  /\ (forall ofs p, Mem.perm m b ofs p -> ofs = 0 /\ p = Nonempty).
-Proof.
-  intros. rewrite find_funct_ptr_iff in H.
-  exploit init_mem_characterization_gen; eauto.
-Qed.
-*)
-
+      
       (** Alignment properties *)
 
       Definition init_data_alignment (i: init_data) : Z :=
